

$$f(x)=\sum_{n=0}^{\infty}\frac{f^{(n)}(a)}{n!}(x-a)^n$$

$$x^n+y^n=z^n$$

$$\frac{(x-x_0)^2}{a^2}+\frac{(y-y_0)^2}{b^2}+\frac{(z-z_0)^2}{c^2}=1$$

$$\varepsilon = \frac{\sqrt{a^2+b^2}}{a}$$

$$\int \sec(ax)dx = \frac{1}{a}\ln\left|\tan\left(\frac{ax}{2}+\frac{\pi}{4}\right)\right|+c$$

$$e^{-at}\sin(\Omega t)u(t)\Leftrightarrow \frac{\Omega}{(s+a)^2+\Omega^2}$$

$$-\frac{\hbar^2}{2m}\frac{\partial^2\psi(x,t)}{\partial x^2}+U(x)\psi(x,t)=i\hbar\frac{\partial\psi(x,t)}{\partial t}$$

$$y=\frac{1}{\sqrt{2\pi}}e^{-\frac{z^2}{2}}=.3989e^{-5z^2}$$

$$e=\lim_{n\rightarrow\infty}\left(1+\frac{1}{n}\right)^n$$

$$\Gamma\left(a\right)=\int\limits_0^{\infty}s^{a-1}e^{-s}ds$$

$$\lim_{x\rightarrow c}\frac{f\left(x\right)}{g\left(x\right)}=\lim_{x\rightarrow c}\frac{f'\left(x\right)}{g'\left(x\right)}$$

$$\lim_{x\rightarrow-\infty}\tan^{-1}\left(x\right)=-\frac{\pi}{2}$$

$$y(x,t)=A_n\cos(\omega_nt+\delta_n)\sin(k_nx)$$

$$A=\frac{F_0}{\sqrt{m^2\left(\omega_0^2-\omega^2\right)^2+b^2\omega^2}}$$

$$E_n=-R_H\left(\frac{1}{n^2}\right)=\frac{-2.178\times10^{-18}}{n^2}joule$$

$$h(n)x(n)\Leftrightarrow \frac{1}{2\pi j}\oint_C H\left(v\right)X\left(z/v\right)v^{-1}dv$$